theories/ml_toy_lang/melocoton/derived_laws.v
@@ -397,4 +397,4 @@ Qed.
 *)
 End lifting.
 
-Typeclasses Opaque array.
+Global Typeclasses Opaque array.
